libcrux-ml-kem/proofs/fstar/extraction/Libcrux_ml_kem.Vector.Portable.Serialize.fsti
@@ -6,92 +6,57 @@ open FStar.Mul
 val deserialize_10_int (bytes: t_Slice u8)
     : Prims.Pure (i16 & i16 & i16 & i16 & i16 & i16 & i16 & i16)
       (requires Core.Slice.impl__len #u8 bytes =. sz 10)
-      (ensures
-        fun tuple ->
-          let tuple:(i16 & i16 & i16 & i16 & i16 & i16 & i16 & i16) = tuple in
-          BitVecEq.int_t_array_bitwise_eq' (bytes <: t_Array _ (sz 10)) 8 (MkSeq.create8 tuple) 10 /\
-          (forall i. Rust_primitives.bounded (Seq.index (MkSeq.create8 tuple) i) 10))
+      (fun _ -> Prims.l_True)
 
 val deserialize_11_int (bytes: t_Slice u8)
     : Prims.Pure (i16 & i16 & i16 & i16 & i16 & i16 & i16 & i16)
       (requires Core.Slice.impl__len #u8 bytes =. sz 11)
-      (ensures
-        fun tuple ->
-          let tuple:(i16 & i16 & i16 & i16 & i16 & i16 & i16 & i16) = tuple in
-          BitVecEq.int_t_array_bitwise_eq' (bytes <: t_Array _ (sz 11)) 8 (MkSeq.create8 tuple) 11 /\
-          (forall i. Rust_primitives.bounded (Seq.index (MkSeq.create8 tuple) i) 11))
+      (fun _ -> Prims.l_True)
 
 val deserialize_12_int (bytes: t_Slice u8)
     : Prims.Pure (i16 & i16)
       (requires Core.Slice.impl__len #u8 bytes =. sz 3)
-      (ensures
-        fun tuple ->
-          let tuple:(i16 & i16) = tuple in
-          BitVecEq.int_t_array_bitwise_eq' (bytes <: t_Array _ (sz 3)) 8 (MkSeq.create2 tuple) 12 /\
-          (forall i. Rust_primitives.bounded (Seq.index (MkSeq.create2 tuple) i) 12))
+      (fun _ -> Prims.l_True)
 
 val deserialize_4_int (bytes: t_Slice u8)
     : Prims.Pure (i16 & i16 & i16 & i16 & i16 & i16 & i16 & i16)
       (requires Core.Slice.impl__len #u8 bytes =. sz 4)
-      (ensures
-        fun tuple ->
-          let tuple:(i16 & i16 & i16 & i16 & i16 & i16 & i16 & i16) = tuple in
-          BitVecEq.int_t_array_bitwise_eq' (bytes <: t_Array _ (sz 4)) 8 (MkSeq.create8 tuple) 4 /\
-          (forall i. Rust_primitives.bounded (Seq.index (MkSeq.create8 tuple) i) 4))
+      (fun _ -> Prims.l_True)
 
 val deserialize_5_int (bytes: t_Slice u8)
     : Prims.Pure (i16 & i16 & i16 & i16 & i16 & i16 & i16 & i16)
       (requires Core.Slice.impl__len #u8 bytes =. sz 5)
-      (ensures
-        fun tuple ->
-          let tuple:(i16 & i16 & i16 & i16 & i16 & i16 & i16 & i16) = tuple in
-          BitVecEq.int_t_array_bitwise_eq' (bytes <: t_Array _ (sz 5)) 8 (MkSeq.create8 tuple) 5 /\
-          (forall i. Rust_primitives.bounded (Seq.index (MkSeq.create8 tuple) i) 4))
+      (fun _ -> Prims.l_True)
 
 val serialize_10_int (v: t_Slice i16)
     : Prims.Pure (u8 & u8 & u8 & u8 & u8)
-      (requires (Core.Slice.impl__len #i16 v <: usize) =. sz 4)
-      (ensures
-        fun tuple ->
-          let tuple:(u8 & u8 & u8 & u8 & u8) = tuple in
-          BitVecEq.int_t_array_bitwise_eq' (v <: t_Array _ (sz 4)) 10 (MkSeq.create5 tuple) 8)
+      (requires Core.Slice.impl__len #i16 v =. sz 4)
+      (fun _ -> Prims.l_True)
 
 val serialize_11_int (v: t_Slice i16)
     : Prims.Pure (u8 & u8 & u8 & u8 & u8 & u8 & u8 & u8 & u8 & u8 & u8)
-      (requires
-        Core.Slice.impl__len #i16 v =. sz 8 /\
-        (forall i. Rust_primitives.bounded (Seq.index v i) 11))
-      (ensures
-        fun tuple ->
-          let tuple:(u8 & u8 & u8 & u8 & u8 & u8 & u8 & u8 & u8 & u8 & u8) = tuple in
-          BitVecEq.int_t_array_bitwise_eq' (v <: t_Array _ (sz 8)) 11 (MkSeq.create11 tuple) 8)
+      (requires Core.Slice.impl__len #i16 v =. sz 8)
+      (fun _ -> Prims.l_True)
 
 val serialize_12_int (v: t_Slice i16)
     : Prims.Pure (u8 & u8 & u8)
-      (requires
-        Core.Slice.impl__len #i16 v =. sz 2 /\
-        (forall i. Rust_primitives.bounded (Seq.index v i) 12))
-      (ensures
-        fun tuple ->
-          let tuple:(u8 & u8 & u8) = tuple in
-          BitVecEq.int_t_array_bitwise_eq' (v <: t_Array _ (sz 2)) 12 (MkSeq.create3 tuple) 8)
+      (requires Core.Slice.impl__len #i16 v =. sz 2)
+      (fun _ -> Prims.l_True)
 
 val serialize_4_int (v: t_Slice i16)
     : Prims.Pure (u8 & u8 & u8 & u8)
-      (requires
-        Core.Slice.impl__len #i16 v =. sz 8 /\ (forall i. Rust_primitives.bounded (Seq.index v i) 4)
-      )
+      (requires Core.Slice.impl__len #i16 v =. sz 8)
       (fun _ -> Prims.l_True)
 
 val serialize_5_int (v: t_Slice i16)
     : Prims.Pure (u8 & u8 & u8 & u8 & u8)
-      (requires
-        Core.Slice.impl__len #i16 v =. sz 8 /\ (forall i. Rust_primitives.bounded (Seq.index v i) 5)
-      )
-      (ensures
-        fun tuple ->
-          let tuple:(u8 & u8 & u8 & u8 & u8) = tuple in
-          BitVecEq.int_t_array_bitwise_eq' (v <: t_Array _ (sz 8)) 5 (MkSeq.create5 tuple) 8)
+      (requires Core.Slice.impl__len #i16 v =. sz 8)
+      (fun _ -> Prims.l_True)
+
+val deserialize_4_ (bytes: t_Slice u8)
+    : Prims.Pure Libcrux_ml_kem.Vector.Portable.Vector_type.t_PortableVector
+      (requires Core.Slice.impl__len #u8 bytes =. sz 8)
+      (fun _ -> Prims.l_True)
 
 val serialize_1_ (v: Libcrux_ml_kem.Vector.Portable.Vector_type.t_PortableVector)
     : Prims.Pure (t_Array u8 (sz 2)) Prims.l_True (fun _ -> Prims.l_True)
@@ -113,30 +78,25 @@ val serialize_5_ (v: Libcrux_ml_kem.Vector.Portable.Vector_type.t_PortableVector
 
 val deserialize_1_ (v: t_Slice u8)
     : Prims.Pure Libcrux_ml_kem.Vector.Portable.Vector_type.t_PortableVector
-      Prims.l_True
+      (requires Core.Slice.impl__len #u8 v =. sz 2)
       (fun _ -> Prims.l_True)
 
 val deserialize_10_ (bytes: t_Slice u8)
     : Prims.Pure Libcrux_ml_kem.Vector.Portable.Vector_type.t_PortableVector
-      Prims.l_True
+      (requires Core.Slice.impl__len #u8 bytes =. sz 20)
       (fun _ -> Prims.l_True)
 
 val deserialize_11_ (bytes: t_Slice u8)
     : Prims.Pure Libcrux_ml_kem.Vector.Portable.Vector_type.t_PortableVector
-      Prims.l_True
+      (requires Core.Slice.impl__len #u8 bytes =. sz 22)
       (fun _ -> Prims.l_True)
 
 val deserialize_12_ (bytes: t_Slice u8)
     : Prims.Pure Libcrux_ml_kem.Vector.Portable.Vector_type.t_PortableVector
-      Prims.l_True
-      (fun _ -> Prims.l_True)
-
-val deserialize_4_ (bytes: t_Slice u8)
-    : Prims.Pure Libcrux_ml_kem.Vector.Portable.Vector_type.t_PortableVector
-      Prims.l_True
+      (requires Core.Slice.impl__len #u8 bytes =. sz 24)
       (fun _ -> Prims.l_True)
 
 val deserialize_5_ (bytes: t_Slice u8)
     : Prims.Pure Libcrux_ml_kem.Vector.Portable.Vector_type.t_PortableVector
-      Prims.l_True
+      (requires Core.Slice.impl__len #u8 bytes =. sz 10)
       (fun _ -> Prims.l_True)
